Proved none and half of alloc

Core.v
@@ -332,10 +332,6 @@ Inductive well_typed_term : ctx -> tm -> typ -> Prop :=
 
   where "Gamma '|--' t 'is' T" := (well_typed_term Gamma t T).
 
-Definition WellTypedTerm (t : tm) := exists T, empty |-- t is T.
-
-Definition WellTypedThread := WellTypedTerm.
-
 (* ------------------------------------------------------------------------- *)
 (* Decidability                                                              *)
 (* ------------------------------------------------------------------------- *)
@@ -370,6 +366,8 @@ Definition forall_memory (m : mem) P : Prop :=
 
 Definition forall_threads (ths : threads) P : Prop :=
   forall_array TM_Unit P ths.
+
+Definition well_typed_thread := fun t => exists T, empty |-- t is T.
 
 (* ------------------------------------------------------------------------- *)
 (* Determinism                                                               *)
